classTable.v
@@ -1,41 +1,24 @@
 Require Import syntax.
 Require Import partial.
+Require Import namesAndTypes.
 Require Import Coq.Structures.Equalities.
 
-Module Type AbstractClassTable (VarNameM FieldNameM MethodNameM ClassNameM: Typ)
-       (v1: Nice VarNameM)
-       (v2: Nice FieldNameM)
-       (v3: Nice MethodNameM)
-       (v4: Nice ClassNameM).
+Module Type AbstractClassTable (ant: AbstractNamesAndTypes).
 
-  Module syn := Syntax VarNameM FieldNameM MethodNameM ClassNameM
-                       v1 v2 v3 v4.
+  Module syn := Syntax ant.
 
   Parameter CT: list syn.ClassDecl.
 End AbstractClassTable.
 
-Module ConcreteClassTable  (VarNameM FieldNameM MethodNameM ClassNameM: Typ)
-       (v1: Nice VarNameM)
-       (v2: Nice FieldNameM)
-       (v3: Nice MethodNameM)
-       (v4: Nice ClassNameM)  <:
-  AbstractClassTable VarNameM FieldNameM MethodNameM
-                     ClassNameM v1 v2 v3 v4.
-  Module syn := Syntax VarNameM FieldNameM MethodNameM ClassNameM
-                       v1 v2 v3 v4.
+Module ConcreteClassTable  (ant: AbstractNamesAndTypes).
+  Module syn := Syntax ant.
   Definition CT := @nil syn.ClassDecl.
 End ConcreteClassTable.  
 
-Module ClassTable (VarNameM FieldNameM MethodNameM ClassNameM: Typ)
-       (act: AbstractClassTable)
-       (v1: Nice VarNameM)
-       (v2: Nice FieldNameM)
-       (v3: Nice MethodNameM)
-       (v4: Nice ClassNameM).
+Module ClassTable (ant: AbstractNamesAndTypes) (act: AbstractClassTable ant).
 
-  Module syn := Syntax VarNameM FieldNameM MethodNameM ClassNameM
-                       v1 v2 v3 v4.
-  Import syn.
+  
+  Import act.syn.
 
   (* Parameter CT : list ClassDecl. *)
   (* Maybe change to method name? *)
@@ -47,8 +30,17 @@ Module ClassTable (VarNameM FieldNameM MethodNameM ClassNameM: Typ)
   
   Definition fld : ClassName -> FieldName -> Prop :=
     fun _ _ => False.
+
+  Definition ftype : forall C f,
+                       fld C f -> ClassName.
+    destruct (ant.fn.constructFresh nil).
+    auto.
+  Defined.
   
   Definition fields : ClassName -> list FieldName -> Prop :=
+    fun _ _ => False.
+
+  Definition subclass : ClassName -> ClassName -> Prop :=
     fun _ _ => False.
 
 End ClassTable.
