namesAndTypes.v
@@ -5,12 +5,36 @@ Require Import Coq.Structures.Equalities.
 Module Type Nice (T: Typ) :=
   (MyDecidableType T) <+ (Infinite T).
 
-Module Type AbstractNamesAndTypes (VarNameM FieldNameM MethodNameM ClassNameM : Typ)
-       (v1: Nice VarNameM)
-       (v2: Nice FieldNameM)
-       (v3: Nice MethodNameM)
-       (v4: Nice ClassNameM).
+Module Type AbstractNamesAndTypes.
+  Declare Module VarNameM : Typ.
+  Declare Module FieldNameM : Typ.
+  Declare Module MethodNameM : Typ.
+  Declare Module ClassNameM : Typ.
+  Declare Module RefM : Typ.
+  Declare Module vn : Nice VarNameM.
+  Declare Module fn : Nice FieldNameM.
+  Declare Module mn : Nice MethodNameM.
+  Declare Module cn : Nice ClassNameM.
+  Declare Module rn : Nice RefM.
 End AbstractNamesAndTypes.
 
-Print AbstractNamesAndTypes.
-Module 
+
+Module ConcreteNamesAndTypes <: AbstractNamesAndTypes.
+  Module VarNameM := natT.
+  Module FieldNameM := natT.
+  Module MethodNameM := natT.
+  Module ClassNameM := natT.
+  Module RefM := natT.
+
+  Module natNice <: Nice natT.
+    Definition eq_dec := nat_eq_dec.
+    Definition constructFresh := infiniteNat.constructFresh.
+  End natNice.
+
+  Module vn := natNice.
+  Module fn := natNice.
+  Module mn := natNice.
+  Module cn := natNice.
+  Module rn := natNice.
+End ConcreteNamesAndTypes.
+
