makefile
@@ -1,6 +1,4 @@
-all:
-	coqc partial.v
-	coqc syntax.v
-	coqc classTable.v
-	coqc heap.v
-	coqc sframe.v
+all: partial.vo namesAndTypes.vo syntax.vo classTable.vo heap.vo sframe.vo reductions.vo typing.vo
+
+%.vo: %.v
+	coqc $^
